@prefix rdf: <http://www.w3.org/1999/02/22-rdf-syntax-ns#> .
@prefix rdfs: <http://www.w3.org/2000/01/rdf-schema#> .
@prefix owl: <http://www.w3.org/2002/07/owl#> .
@prefix dcterms: <http://purl.org/dc/terms/> .

<http://open-services.net/ns/basicProfile#> a owl:Ontology ;
	dcterms:title "The Linked Data Basic Profile (LDBP) Vocabulary" ;
	dcterms:description "All vocabulary URIs defined in the Linked Data Basic Profile (LDBP) namespace." ;
	rdfs:label "Linked Data Basic Profile (LDBP)" ;
	rdfs:seeAlso <http://www.w3.org/2011/09/LinkedData/> , <http://www.ibm.com/developerworks/rational/library/basic-profile-linked-data/> , <http://open-services.net/ns/basicProfile/ldbp.rdf> .

<http://open-services.net/ns/basicProfile#Container> a rdfs:Class ;
	rdfs:isDefinedBy <http://open-services.net/ns/basicProfile#> ;
	rdfs:label "Container" ;
	rdfs:comment """A Basic Profile Resource (BPR) that also conforms to additional patterns 
		and conventions in this document for managing membership.""" .

<http://open-services.net/ns/basicProfile#Page> a rdfs:Class ;
	rdfs:isDefinedBy <http://open-services.net/ns/basicProfile#> ;
	rdfs:label "Page" ;
	rdfs:comment "A resource that represents a limited set of members of a Basic Profile Container." .

<http://open-services.net/ns/basicProfile#membershipPredicate> a rdf:Property ;
	rdfs:isDefinedBy <http://open-services.net/ns/basicProfile#> ;
	rdfs:label "membershipPredicate" ;
	rdfs:comment "Indicates which predicate of the container should be used to determine the membership." ;
	rdfs:domain <http://open-services.net/ns/basicProfile#Container> ;
	rdfs:range rdf:Property .

<http://open-services.net/ns/basicProfile#membershipSubject> a rdf:Property ;
	rdfs:isDefinedBy <http://open-services.net/ns/basicProfile#> ;
	rdfs:label "membershipSubject" ;
	rdfs:comment "Indicates which resource is the subject for the members of the container." ;
	rdfs:domain <http://open-services.net/ns/basicProfile#Container> ;
	rdfs:range rdf:Property .

<http://open-services.net/ns/basicProfile#pageOf> a rdf:Property ;
	rdfs:isDefinedBy <http://open-services.net/ns/basicProfile#> ;
	rdfs:label "pageOf" ;
	rdfs:comment "Associated a page with its container." ;
	rdfs:domain <http://open-services.net/ns/basicProfile#Page> ;
	rdfs:range <http://open-services.net/ns/basicProfile#Container> .

<http://open-services.net/ns/basicProfile#nextPage> a rdf:Property ;
	rdfs:isDefinedBy <http://open-services.net/ns/basicProfile#> ;
	rdfs:label "nextPage" ;
	rdfs:comment "From a known page, how to indicate the next or last page as rdf:nil." ;
	rdfs:domain <http://open-services.net/ns/basicProfile#Page> ;
	rdfs:range rdfs:Resource .

<http://open-services.net/ns/basicProfile#containerSortPredicates> a rdf:Property ;
	rdfs:isDefinedBy <http://open-services.net/ns/basicProfile#> ;
	rdfs:label "containerSortPredicates" ;
	rdfs:comment "List of predicates that indicate the ascending order of the members in a page." ;
	rdfs:domain <http://open-services.net/ns/basicProfile#Page> ;
	rdfs:range rdf:List .